Work on the proof of quorum

Isabelle2/Quorum.thy
@@ -59,7 +59,7 @@ definition init_acc where
     \<and> r' = r\<lparr>acc_status := (acc_status r)(p := Ready), acc_cstruct := (acc_cstruct r)(p := s)\<rparr>"
 
 definition accept where
-  "accept r r' \<equiv> \<exists> p . \<exists> c \<in> q_state.propCmd r .
+  "accept r r' \<equiv> \<exists> p \<in> acceptors . \<exists> c \<in> q_state.propCmd r .
     acc_status r p = Ready
     \<and> r' = r\<lparr>acc_status := (acc_status r)(p := Ready), 
         acc_cstruct := (acc_cstruct r)(p := acc_cstruct r p \<bullet> c)\<rparr>"
@@ -156,6 +156,16 @@ definition inv2 where
   "inv2 r \<equiv> \<forall> p \<in> acceptors . q_state.acc_status r p \<noteq> Idle \<longrightarrow> \<Sqinter> (q_state.from_prev r) \<preceq> acc_cstruct r p"
 declare inv2_def[inv_defs]
 
+definition inv3 where
+  "inv3 r \<equiv> finite (q_state.from_prev r) \<and> finite (q_state.to_next r)"
+declare inv3_def[inv_defs]
+
+lemma inv3:"invariant q_ioa inv3"
+apply try_solve_inv
+apply auto
+done
+declare inv3[invs]
+
 lemma inv1:"invariant q_ioa inv1"
 apply try_solve_inv
 subgoal by auto
@@ -166,16 +176,35 @@ declare inv1[invs]
 
 lemma inv2:"invariant q_ioa inv2"
 apply try_solve_inv
-subgoal by clarify (meson glb_anti pre_CStruct.trans)
+subgoal by clarify (meson glb_insert pre_CStruct.trans)
 subgoal premises prems for s t a x
   -- "TODO: here we would need some method instantiating exI"
   proof -
   from prems(2) have "\<exists> p \<in> acceptors  . acc_status s p \<noteq> Idle" by force
-  hence "q_state.from_prev s \<noteq> {}" using prems(3) by blast
+  hence "q_state.from_prev s \<noteq> {}" using prems(4) by blast
   with glb_anti and prems show ?thesis apply clarsimp
   by (metis acc_status.distinct(1)) 
   qed
-
+subgoal premises prems for s t a
+  proof auto
+  fix p
+  assume 1:"p \<in> acceptors" and 2:"acc_status t p \<noteq> Idle"
+  from prems(2) obtain q cstr where 3:"acc_status s q = Idle \<and>
+    cstr \<in> q_state.from_prev s \<and> t = s\<lparr>acc_status := (acc_status s)(q := Ready),
+      acc_cstruct := (acc_cstruct s)(q := cstr)\<rparr>" by blast
+  from 1 2 3 prems(1,3,4,5) glb_anti show "\<Sqinter> q_state.from_prev t \<preceq> acc_cstruct t p" 
+  by(clarsimp, insert coboundedI, auto)
+  qed
+subgoal premises prems for s t a
+  proof -
+  obtain p c where 1:"p \<in> acceptors \<and> acc_status s p \<noteq> Idle 
+    \<and> t = s\<lparr>acc_status := (acc_status s)(p := Ready),
+            acc_cstruct := (acc_cstruct s)(p := acc_cstruct s p \<bullet> c)\<rparr>" using prems(2) by force
+  from 1 prems(1) show "\<forall>p\<in>acceptors. acc_status t p \<noteq> Idle \<longrightarrow>
+    \<Sqinter> q_state.from_prev t \<preceq> acc_cstruct t p" 
+    by auto (metis less_bullet pre_CStruct.trans) 
+  qed
+done
 
 lemma refok:"is_ref_map refmap q_ioa spec" 
 apply(simp add:is_ref_map_def refmap_def, rule conjI; clarify)
